tla-tree/CrashSafeTreeInv.dfy
@@ -1,6 +1,103 @@
 include "CrashSafeTree.dfy"
 
 module CrashSafeTreeInv {
-import TreeDisk
+import opened CrashSafeTree
+
+predicate IsNodeStorage(lba:LBA, super:Sector)  // Trigger target.
+    requires super.Superblock?
+{
+    1 <= lba < super.virgin
+}
+
+predicate MinimalDisk(k:Constants)
+{
+    2 <= k.disk.size
+}
+
+predicate DiskStructureInv(k:Constants, s:Variables)
+    requires TreeDisk.WF(k.disk, s.disk)
+    requires MinimalDisk(k)
+{
+    && 1 <= k.disk.size // Gotta have room for a superblock!
+    && var super := TreeDisk.PeekF(k.disk, s.disk, SUPERBLOCK_LBA());
+    && super.Superblock?
+    && super.virgin <= k.disk.size   // used blocks fit on the disk
+    && (forall lba :: IsNodeStorage(lba, super) ==>
+            !TreeDisk.PeekF(k.disk, s.disk, lba).Superblock?
+        )
+}
+
+predicate CacheEntryReflectsDisk(k:Constants, s:Variables, lba:LBA)
+    requires TreeDisk.WF(k.disk, s.disk)
+    requires lba in s.cache
+{
+    && TreeDisk.ValidLBA(k.disk, lba)
+    && s.cache[lba] == TreeDisk.PeekF(k.disk, s.disk, lba)
+}
+
+predicate CacheReflectsDisk(k:Constants, s:Variables)
+    requires TreeDisk.WF(k.disk, s.disk)
+{
+    forall lba :: lba in s.cache ==> CacheEntryReflectsDisk(k, s, lba)
+}
+
+predicate Inv(k:Constants, s:Variables)
+{
+    && TreeDisk.WF(k.disk, s.disk)
+    && MinimalDisk(k)
+    && DiskStructureInv(k, s)
+    && CacheReflectsDisk(k, s)
+}
+
+lemma InvHoldsInit(k:Constants, s:Variables)
+    requires Init(k, s)
+    ensures Inv(k, s)
+{
+    var super := TreeDisk.PeekF(k.disk, s.disk, SUPERBLOCK_LBA());
+    forall lba | IsNodeStorage(lba, super)
+        ensures !TreeDisk.PeekF(k.disk, s.disk, lba).Superblock?
+    {
+        assert lba == 1;
+    }
+}
+
+lemma InvHoldsInduction(k:Constants, s:Variables, s':Variables)
+    requires Inv(k, s)
+    requires Next(k, s, s')
+    ensures Inv(k, s')
+{
+    var step :| NextStep(k, s, s', step);
+    match step {
+        case CacheFaultActionStep(lba, sector) => {
+            assert DiskStructureInv(k, s');
+        }
+        case CacheEvictActionStep(lba) => {
+            assert DiskStructureInv(k, s');
+        }
+        case PrepareGrowActionStep(parentRead, i, childRead) => {
+            assert DiskStructureInv(k, s');
+        }
+        case CommitGrowActionStep(parentRead, i, childRead) => {
+            assert DiskStructureInv(k, s');
+        }
+        case ContractNodeActionStep(parentRead, i, childRead) => {
+            assert DiskStructureInv(k, s');
+        }
+        case QueryActionStep(datum, lookup) => {
+        }
+        case InsertActionStep(datum, lookup) => {
+            assert DiskStructureInv(k, s');
+        }
+        case DeleteActionStep(datum, lookup) => {
+            assert DiskStructureInv(k, s');
+        }
+        case MoveToFreeListActionStep(lba, childRead) => {
+            assert DiskStructureInv(k, s');
+        }
+        case CommitFreeListActionStep(super) => {
+            assert DiskStructureInv(k, s');
+        }
+    }
+}
 
 }
